
{-# OPTIONS --without-K --safe #-}
-- https://www.cs.bham.ac.uk/~mhe/papers/omniscient-journal-revised.pdf

module Constructive.OmniscienceAlt where

open import Level renaming (zero to lzero; suc to lsuc)
import Data.Bool as ğ”¹ using (_â‰¤_)
open import Data.Bool as ğ”¹ using (Bool; true; false; T; fâ‰¤t; bâ‰¤b; _âˆ§_; not; _âˆ¨_)
import Data.Bool.Properties as ğ”¹â‚š
open import Data.Empty
open import Data.Unit using (tt)
open import Data.Nat
open import Data.Nat.Properties
open import Data.Product as Prod
open import Data.Sum as Sum
open import Function.Base
open import Relation.Binary as B
open import Relation.Binary.PropositionalEquality
open import Relation.Nullary
open import Relation.Nullary.Decidable
import Relation.Unary as U

-- agda-misc
open import Constructive.Axiom
open import Constructive.Axiom.Properties
open import Constructive.Axiom.Properties.Base.Lemma
open import Constructive.Common
open import Constructive.Combinators

â„•âˆ : Set
â„•âˆ = Î£ (â„• â†’ Bool) Î» x â†’ âˆ€ i â†’ T (x i) â†’ T (x (suc i))

fromâ„•-C : â„• â†’ â„• â†’ Bool
fromâ„•-C zero    zero    = false
fromâ„•-C zero    (suc n) = true
fromâ„•-C (suc m) zero    = false
fromâ„•-C (suc m) (suc n) = fromâ„•-C m n

fromâ„•-convergent : âˆ€ n i â†’ T (fromâ„•-C n i) â†’ T (fromâ„•-C n (suc i))
fromâ„•-convergent zero    (suc i) t = tt
fromâ„•-convergent (suc n) (suc i) t = fromâ„•-convergent n i t

fromâ„• : â„• â†’ â„•âˆ
fromâ„• n = fromâ„•-C n , fromâ„•-convergent n

âˆ : â„•âˆ
âˆ = (Î» _ â†’ false) , (Î» i x â†’ x)

_â‰ˆ_ : Rel (â„• â†’ Bool) lzero
Î± â‰ˆ Î² = âˆ€ i â†’ Î± i â‰¡ Î² i

_â‰‰_ : Rel (â„• â†’ Bool) lzero
Î± â‰‰ Î² = Â¬ (Î± â‰ˆ Î²)

_#_ : Rel (â„• â†’ Bool) lzero
Î± # Î² = âˆƒ Î» i â†’ Î± i â‰¢ Î² i

#â‡’â‰‰  : {Î± Î² : â„• â†’ Bool} â†’ Î± # Î² â†’ Î± â‰‰ Î²
#â‡’â‰‰ {Î±} {Î²} (i , Î±iâ‰¢Î²i) Î±â‰ˆÎ² = Î±iâ‰¢Î²i (Î±â‰ˆÎ² i)

â‰ˆ-refl : {Î± : â„• â†’ Bool} â†’ Î± â‰ˆ Î±
â‰ˆ-refl _ = refl

â‰ˆ-sym : {Î± Î² : â„• â†’ Bool} â†’ Î± â‰ˆ Î² â†’ Î² â‰ˆ Î±
â‰ˆ-sym Î±â‰ˆÎ² i = sym (Î±â‰ˆÎ² i)

â‰ˆ-trans : {Î± Î² Î³ : â„• â†’ Bool} â†’ Î± â‰ˆ Î² â†’ Î² â‰ˆ Î³ â†’ Î± â‰ˆ Î³
â‰ˆ-trans Î±â‰ˆÎ² Î²â‰ˆÎ³ i = trans (Î±â‰ˆÎ² i) (Î²â‰ˆÎ³ i)

_â‰ˆâˆ_ : Rel â„•âˆ lzero
x â‰ˆâˆ y = projâ‚ x â‰ˆ projâ‚ y

_â‰‰âˆ_ : Rel â„•âˆ lzero
x â‰‰âˆ y = projâ‚ x â‰‰ projâ‚ y

_#âˆ_ : Rel â„•âˆ lzero
x #âˆ y = projâ‚ x # projâ‚ y

-- Proposition 3.1
-- r = â‰¤-any

â‰¤-any : (â„• â†’ Bool) â†’ (â„• â†’ Bool)
â‰¤-any Î± zero    = Î± 0
â‰¤-any Î± (suc n) = Î± (suc n) âˆ¨ â‰¤-any Î± n

â‰¤-any-idem : âˆ€ Î± â†’ â‰¤-any (â‰¤-any Î±) â‰ˆ â‰¤-any Î±
â‰¤-any-idem Î± zero    = refl
â‰¤-any-idem Î± (suc n) = begin
  (Î± (suc n) âˆ¨ â‰¤-any Î± n) âˆ¨ â‰¤-any (â‰¤-any Î±) n
    â‰¡âŸ¨ cong ((Î± (suc n) âˆ¨ â‰¤-any Î± n) âˆ¨_) $ â‰¤-any-idem Î± n âŸ©
  (Î± (suc n) âˆ¨ â‰¤-any Î± n) âˆ¨ â‰¤-any Î± n
    â‰¡âŸ¨ ğ”¹â‚š.âˆ¨-assoc (Î± (suc n)) (â‰¤-any Î± n) (â‰¤-any Î± n) âŸ©
  Î± (suc n) âˆ¨ (â‰¤-any Î± n âˆ¨ â‰¤-any Î± n)
    â‰¡âŸ¨ cong (Î± (suc n) âˆ¨_) $ ğ”¹â‚š.âˆ¨-idem (â‰¤-any Î± n) âŸ©
  Î± (suc n) âˆ¨ â‰¤-any Î± n
    âˆ
  where open â‰¡-Reasoning

private
  T-âˆ§-Ã— : âˆ€ {x y} â†’ T (x âˆ§ y) â†’ (T x Ã— T y)
  T-âˆ§-Ã— {true} {true} t = tt , tt

  T-Ã—-âˆ§ : âˆ€ {x y} â†’ (T x Ã— T y) â†’ T (x âˆ§ y)
  T-Ã—-âˆ§ {true} {true} (tt , tt) = tt

  T-âˆ¨-introÊ³ : âˆ€ {x y} â†’ T y â†’ T (x âˆ¨ y)
  T-âˆ¨-introÊ³ {true} {true} t = tt
  T-âˆ¨-introÊ³ {false} {true} t = tt

  T-âˆ¨-introË¡ : âˆ€ {x y} â†’ T x â†’ T (x âˆ¨ y)
  T-âˆ¨-introË¡ {true} {true} t = tt
  T-âˆ¨-introË¡ {true} {false} t = tt

â‰¤-any-convergent : âˆ€ Î± i â†’ T (â‰¤-any Î± i) â†’ T (â‰¤-any Î± (suc i))
â‰¤-any-convergent Î± n t = T-âˆ¨-introÊ³ t

â‰¤-any-â„•âˆ : (â„• â†’ Bool) â†’ â„•âˆ
â‰¤-any-â„•âˆ Î± = â‰¤-any Î± , â‰¤-any-convergent Î±

â‰¤-any-construct : âˆ€ Î± n â†’ T (Î± n) â†’ T (â‰¤-any Î± n)
â‰¤-any-construct Î± zero    t = t
â‰¤-any-construct Î± (suc n) t = T-âˆ¨-introË¡ t

private
  not-injective : âˆ€ {x y} â†’ not x â‰¡ not y â†’ x â‰¡ y
  not-injective {false} {false} refl = refl
  not-injective {true}  {true}  refl = refl

  xâ‰¢yâ‡’not[x]â‰¡y : âˆ€ {x y} â†’ x â‰¢ y â†’ not x â‰¡ y
  xâ‰¢yâ‡’not[x]â‰¡y {false} {false} xâ‰¢y = contradiction refl xâ‰¢y
  xâ‰¢yâ‡’not[x]â‰¡y {false} {true} xâ‰¢y = refl
  xâ‰¢yâ‡’not[x]â‰¡y {true} {false} xâ‰¢y = refl
  xâ‰¢yâ‡’not[x]â‰¡y {true} {true} xâ‰¢y = contradiction refl xâ‰¢y

  xâ‰¢yâ‡’xâ‰¡not[y] : âˆ€ {x y} â†’ x â‰¢ y â†’ x â‰¡ not y
  xâ‰¢yâ‡’xâ‰¡not[y] {x} {y} xâ‰¢y = subst (_â‰¡ not y) (ğ”¹â‚š.not-involutive x) $
                             xâ‰¢yâ‡’not[x]â‰¡y {not x} {not y} (xâ‰¢y âˆ˜â€² not-injective)

  xâ‰¡yâ‡’not[x]â‰¢y : âˆ€ {x y} â†’ x â‰¡ y â†’ not x â‰¢ y
  xâ‰¡yâ‡’not[x]â‰¢y {false} {false} p ()
  xâ‰¡yâ‡’not[x]â‰¢y {false} {true} () q
  xâ‰¡yâ‡’not[x]â‰¢y {true} {false} () q
  xâ‰¡yâ‡’not[x]â‰¢y {true} {true} p ()

  not[x]â‰¡trueâ†’xâ‰¢true : âˆ€ {x} â†’ not x â‰¡ true â†’ x â‰¢ true
  not[x]â‰¡trueâ†’xâ‰¢true {false} refl ()
  not[x]â‰¡trueâ†’xâ‰¢true {true}  ()   p

  falseâ‰¢true : false â‰¢ true
  falseâ‰¢true ()

lpo-Boolâ‡’âˆ€xâ†’x#âˆâŠxâ‰ˆâˆ : LPO-Bool â„• â†’ âˆ€ x â†’ (x #âˆ âˆ) âŠ (x â‰ˆâˆ âˆ)
lpo-Boolâ‡’âˆ€xâ†’x#âˆâŠxâ‰ˆâˆ lpo-Bool (Î± , con) with lpo-Bool Î±
... | injâ‚ (x , Î±xâ‰¡true) = injâ‚ (x , Î» Î±xâ‰¡false â†’ falseâ‰¢true (trans (sym Î±xâ‰¡false) Î±xâ‰¡true))
... | injâ‚‚ Â¬âˆƒxâ†’Î±xâ‰¡true   = injâ‚‚ Î» i â†’  xâ‰¢yâ‡’xâ‰¡not[y] $â€² Â¬âˆƒPâ†’âˆ€Â¬P Â¬âˆƒxâ†’Î±xâ‰¡true i


T-to-â‰¡ : âˆ€ {x} â†’ T x â†’ x â‰¡ true
T-to-â‰¡ {true} tx = refl

â‰¡-to-T : âˆ€ {x} â†’ x â‰¡ true â†’ T x
â‰¡-to-T {true} xâ‰¡true = tt

private
  T-Â¬-not : âˆ€ {x} â†’ Â¬ (T x) â†’ T (not x)
  T-Â¬-not {false} n = tt
  T-Â¬-not {true}  n = n tt

  T-not-Â¬ : âˆ€ {x} â†’ T (not x) â†’ Â¬ (T x)
  T-not-Â¬ {false} tt ()
  T-not-Â¬ {true}  () y

Â¬T-â‰¤-any : âˆ€ Î± x â†’ Â¬ T (â‰¤-any Î± x) â†’ âˆƒ Î» y â†’ Â¬ T (Î± y)
Â¬T-â‰¤-any Î± zero    Â¬T with Î± 0 | inspect Î± 0
... | true  | [ Î±0â‰¡true ]  = contradiction tt Â¬T
... | false | [ Î±0â‰¡false ] = zero , (Î» T[Î±0] â†’ subst T Î±0â‰¡false T[Î±0])
Â¬T-â‰¤-any Î± (suc x) Â¬T with Î± (suc x) | inspect Î± (suc x)
... | true  | [ Î±snâ‰¡true ] = Â¬T-â‰¤-any Î± x Â¬T
... | false | [ Î±snâ‰¡false ] = (suc x) , (Î» T[Î±sn] â†’ subst T Î±snâ‰¡false T[Î±sn])
{-
Â¬T-â‰¤-anyâ€² : âˆ€ Î± x â†’ Â¬ T (â‰¤-any (not âˆ˜â€² Î±) x) â†’ âˆƒ Î» y â†’ T (Î± y)
Â¬T-â‰¤-anyâ€² Î± x Â¬T =
  Prod.mapâ‚‚ (Î» nt â†’ subst T (ğ”¹â‚š.not-involutive _) (T-Â¬-not nt)) $â€²
  Â¬T-â‰¤-any (not âˆ˜ Î±) x Â¬T

âˆ€xâ†’x#âˆâŠxâ‰ˆâˆâ‡’lpo-Bool : (âˆ€ x â†’ (x #âˆ âˆ) âŠ (x â‰ˆâˆ âˆ)) â†’ LPO-Bool â„•
âˆ€xâ†’x#âˆâŠxâ‰ˆâˆâ‡’lpo-Bool â‰ˆâˆ? P with â‰ˆâˆ? (â‰¤-any-â„•âˆ (Î» n â†’ not (P n)))
... | injâ‚ (x , â‰¤-any[notâˆ˜P,x]â‰¢true) =
  injâ‚ (Prod.mapâ‚‚ T-to-â‰¡ (Â¬T-â‰¤-anyâ€² P x (contraposition T-to-â‰¡ â‰¤-any[notâˆ˜P,x]â‰¢true)))
... | injâ‚‚ âˆ€iâ†’â‰¤-any[notâˆ˜P,i]â‰¡true =
  injâ‚‚ (âˆ€Â¬Pâ†’Â¬âˆƒP Î» i â†’ not[x]â‰¡trueâ†’xâ‰¢true (T-to-â‰¡ $ â‰¤-any-extract (not âˆ˜ P) i $ â‰¡-to-T (âˆ€iâ†’â‰¤-any[notâˆ˜P,i]â‰¡true i)))

--  â‰¤-any (Î» n â†’ not (P n)) x â‰¡ true â†’ âŠ¥
-- â‰¤-any (not âˆ˜ P) x â‰¡ false
--
--  ---------------------------
--  T (â‰¤-any P x)
-}
